compiler/bootstrap/translation/compiler64ProgScript.sml
@@ -264,55 +264,6 @@ val res = format_compiler_result_def
 
 val res = translate compile_64_def;
 
-val res = translate panPtreeConversionTheory.argsNT_def;
-
-val res = translate panPtreeConversionTheory.destLf_def;    
-
-val res = translate panPtreeConversionTheory.destTOK_def;
-
-val res = translate $ PURE_REWRITE_RULE [GSYM implode_def] panPtreeConversionTheory.conv_ident_def;
-
-val res = translate panPtreeConversionTheory.isNT_def;
-
-val res = translate panPtreeConversionTheory.conv_int_def;
-
-Theorem conv_const_thm:
-  conv_const t =
-  case conv_int t of NONE => (NONE:'a panLang$exp option)
-         | SOME x => SOME(Const(i2w x))
-Proof
-  Cases_on ‘conv_int t’ \\ rw[panPtreeConversionTheory.conv_const_def]
-QED
-
-val conv64 = GEN_ALL o CONV_RULE (wordsLib.WORD_CONV) o spec64 o SPEC_ALL        
-val res = translate $ spec64 conv_const_thm;        
-        
-Definition conv_c_thm:
-  conv_ct t =
-  case conv_int t of NONE => (NONE:'a wordLang$exp option)
-         | SOME x => SOME(Const(i2w x))
-End
-
-Definition conv_cd_thm:
-  conv_cd t =
-  case conv_int t of NONE => (NONE:'a panLang$exp option)
-         | SOME x => SOME(Const(i2w x))
-End                        
-
-val res = translate $ spec64 conv_cd_thm;
-                   
-val res = translate $ conv64 conv_const_thm;
-
-val res = translate panPtreeConversionTheory.conv_nat_def;
-    
-val res = translate $ INST_TYPE[beta|->``:64``] panPtreeConversionTheory.conv_Exp_def;
-
-val res = translate $ INST_TYPE[beta|->``:64``] panPtreeConversionTheory.conv_NonRecStmt_def;
-
-val res = translate $ spec64 panPtreeConversionTheory.conv_Prog_def;
-    
-val res = translate $ spec64 panPtreeConversionTheory.parse_to_ast_def;
-    
 val res = translate $ spec64 compile_pancake_def;
     
 val res = translate compile_pancake_64_def;
@@ -519,9 +470,8 @@ End
 val _ = (next_ml_names := ["compiler_has_repl_flag"]);
 val res = translate (has_repl_flag_def |> REWRITE_RULE [MEMBER_INTRO]);
 
-val _ = (next_ml_names := ["compiler_has_pancake_flag"]);
-val res = translate (has_pancake_flag_def |> REWRITE_RULE [MEMBER_INTRO]);
-    
+val res = translate (has_pancake_flag_def |> SIMP_RULE (srw_ss()) [MEMBER_INTRO])
+
 val main = process_topdecs`
   fun main u =
     let
@@ -533,10 +483,11 @@ val main = process_topdecs`
         print compiler_help_string
       else if compiler_has_version_flag cl then
         print compiler_current_build_info_str
-      else if compiler_has_pancake_flag
-        case compiler_compile_64 cl (TextIO.inputAll TextIO.stdIn)  of
+      else if compiler_has_pancake_flag cl then
+        case compiler_compile_pancake_64 cl (TextIO.inputAll TextIO.stdIn)  of
           (c, e) => (print_app_list c; TextIO.output TextIO.stdErr e;
-                     compiler64prog_nonzero_exit_code_for_error_msg e)      else
+                     compiler64prog_nonzero_exit_code_for_error_msg e)
+      else
         case compiler_compile_64 cl (TextIO.inputAll TextIO.stdIn)  of
           (c, e) => (print_app_list c; TextIO.output TextIO.stdErr e;
                      compiler64prog_nonzero_exit_code_for_error_msg e)
@@ -607,6 +558,29 @@ Proof
     \\ CONV_TAC SWAP_EXISTS_CONV
     \\ qexists_tac`fs`
     \\ xsimpl)
+  >> xlet_auto>-xsimpl
+  >> xif
+  >- (
+     xlet_auto >- (xsimpl \\ fs[INSTREAM_stdin, STD_streams_get_mode])
+     \\ fs [GSYM HOL_STRING_TYPE_def]
+     \\ xlet_auto >- xsimpl
+     \\ fs [full_compile_64_def]
+     \\ pairarg_tac
+     \\ fs[ml_translatorTheory.PAIR_TYPE_def]
+     \\ gvs[CaseEq "bool"]
+     \\ xmatch
+     \\ xlet_auto >- xsimpl
+
+     \\ qmatch_goalsub_abbrev_tac `STDIO fs'`
+     \\ xlet `POSTv uv. &UNIT_TYPE () uv * STDIO (add_stderr fs' err) *
+        COMMANDLINE cl`
+     THEN1
+      (xapp_spec output_stderr_spec \\ xsimpl
+       \\ qexists_tac `COMMANDLINE cl`
+       \\ asm_exists_tac \\ xsimpl
+       \\ qexists_tac `fs'` \\ xsimpl)
+     \\ xapp
+     \\ asm_exists_tac \\ simp [] \\ xsimpl)
   \\ xlet_auto >- (xsimpl \\ fs[INSTREAM_stdin, STD_streams_get_mode])
   \\ fs [GSYM HOL_STRING_TYPE_def]
   \\ xlet_auto >- xsimpl
@@ -616,8 +590,6 @@ Proof
   \\ gvs[CaseEq "bool"]
   \\ xmatch
   \\ xlet_auto >- xsimpl
-
-
   \\ qmatch_goalsub_abbrev_tac `STDIO fs'`
   \\ xlet `POSTv uv. &UNIT_TYPE () uv * STDIO (add_stderr fs' err) *
                      COMMANDLINE cl`
